Use `stuck e σ` rather than `¬ progressive e σ`.

theories/program_logic/ectx_language.v
@@ -100,8 +100,8 @@ Section ectx_language.
     ∃ e' σ' efs, head_step e σ e' σ' efs.
   Definition head_irreducible (e : expr Λ) (σ : state Λ) :=
     ∀ e' σ' efs, ¬head_step e σ e' σ' efs.
-  Definition head_progressive (e : expr Λ) (σ : state Λ) :=
-    is_Some(to_val e) ∨ ∃ K e', e = fill K e' ∧ head_reducible e' σ.
+  Definition head_stuck (e : expr Λ) (σ : state Λ) :=
+    to_val e = None ∧ ∀ K e', e = fill K e' → head_irreducible e' σ.
 
   (* All non-value redexes are at the root.  In other words, all sub-redexes are
      values. *)
@@ -165,12 +165,12 @@ Section ectx_language.
     rewrite -not_reducible -not_head_reducible. eauto using prim_head_reducible.
   Qed.
 
-  Lemma progressive_head_progressive e σ :
-    progressive e σ → head_progressive e σ.
+  Lemma head_stuck_stuck e σ :
+    head_stuck e σ → sub_redexes_are_values e → stuck e σ.
   Proof.
-    case=>[?|Hred]; first by left.
-    right. move: Hred=> [] e' [] σ' [] efs [] K e1' e2' EQ EQ' Hstep. subst.
-    exists K, e1'. split; first done. by exists e2', σ', efs.
+    move=>[] ? Hirr ?. split; first done.
+    apply prim_head_irreducible; last done.
+    apply (Hirr empty_ectx). by rewrite fill_empty.
   Qed.
 
   Lemma ectx_language_atomic s e :
